stdlib/ptr/output/ptr/proofs/proof_const_ptr_with_addr.v
@@ -1,0 +1,40 @@
+From caesium Require Import lang notation.
+From refinedrust Require Import typing shims.
+From stdlib.ptr.ptr.generated Require Import generated_code_ptr generated_specs_ptr generated_template_const_ptr_with_addr.
+
+Set Default Proof Using "Type".
+
+Section proof.
+Context `{RRGS : !refinedrustGS Σ}.
+
+Lemma const_ptr_with_addr_proof (π : thread_id) :
+  const_ptr_with_addr_lemma π.
+Proof.
+  const_ptr_with_addr_prelude.
+
+  repeat liRStep; liShow.
+  typed_val_expr_bind.
+  repeat liRStep; liShow.
+  typed_val_expr_bind.
+  repeat liRStep; liShow.
+  rewrite /typed_val_expr.
+  iIntros (?) "#CTX HE HL HCont".
+  iRename select (_ ◁ᵥ{π} addr @ int usize_t)%I into "Hv".
+  iEval (rewrite /ty_own_val/=) in "Hv".
+  iDestruct "Hv" as "[% %]".
+  iApply wp_copy_alloc_id; [done | apply val_to_of_loc | ].
+  iNext. iIntros "_".
+  set (l := (x.1, addr) : loc).
+  iAssert (l ◁ᵥ{π} (x.1, addr) @ alias_ptr_t)%I as "?".
+  { rewrite /ty_own_val/=. iSplitR; first done.
+    simpl. iPureIntro. apply int_elem_of_it_iff. by eapply val_to_Z_in_range. }
+  iApply ("HCont" $! _ π _ _ (alias_ptr_t) l with "HL []").
+  { done. }
+  repeat liRStep; liShow.
+
+  all: print_remaining_goal.
+  Unshelve. all: sidecond_solver.
+  Unshelve. all: sidecond_hammer.
+  Unshelve. all: print_remaining_sidecond.
+Qed.
+End proof.
